hashed_elgamal_generic with existential and without Bound module

examples/hashed_elgamal_generic.ec
@@ -1,6 +1,6 @@
-require import AllCore Int Real FSet.
+require import AllCore FSet List SmtMap.
 require (*--*) BitWord Distr DInterval.
-(*---*) import StdOrder.RealOrder StdRing.RField.
+(*---*) import StdOrder.RealOrder StdRing.RField StdBigop.Bigint BIA.
 require (*--*) DiffieHellman ROM PKE_CPA.
 
 (* The type of plaintexts: bitstrings of length k *)
@@ -14,13 +14,27 @@ rename
   "dunifin" as "dbits".
 import DWord.
 
-(* Upper bound on the number of calls to H *)
-op qH: { int | 0 < qH } as gt0_qH.
+(* Upper bound on complexity of the adversary *)
+type adv_cost = {
+  cchoose : int; (* cost *)
+  ochoose : int; (* number of call to o *)
+  cguess  : int; (* cost *)
+  oguess  : int; (* number of call to o *)
+}.
+
+op cA : adv_cost.
+axiom cA_pos : 0 <= cA.`cchoose /\ 0 <= cA.`ochoose /\ 0 <= cA.`cguess /\ 0 <= cA.`oguess /\ 0 < cA.`ochoose + cA.`oguess.
+
+op qH = cA.`ochoose + cA.`oguess.
+lemma gt0_qH :  0 < qH by smt (cA_pos).
 
 (* Assumption: Set CDH *)
-clone import DiffieHellman.Set_CDH as SCDH with
-  op n <- qH.
+clone import DiffieHellman.List_CDH as LCDHT with
+  op n <- qH
+  proof gt0_n by apply gt0_qH.
 import DiffieHellman G FDistr.
+
+clone import LCDHT.C as C1.
 
 type pkey = group.
 type skey = t.
@@ -66,11 +80,10 @@ module Hashed_ElGamal (H:Hash): Scheme = {
   }
 }.
 
-clone import ROM.ROM_BadCall as ROC with
+clone import ROM.Lazy as ROL with
   type from  <- group,
   type to    <- bits,
-  op dsample <- fun (x:group), dbits,
-  op qH      <- qH
+  op dsample <- fun (x:group), dbits
 proof * by exact/dbits_ll.
 
 (* Adversary Definitions *)
@@ -80,16 +93,19 @@ module type Adversary (O:ARO) = {
 }.
 
 (* Specializing and merging the hash function *)
-module H:Hash = {
-  proc init(): unit = { RO.init(); Log.qs <- fset0; }
-  proc hash(x:group): bits = { var y; y <@ RO.o(x); return y; }
+module H = {
+  var qs : group list
+  proc init(): unit = { RO.init(); qs <- []; }
+  proc o(x:group): bits = { var y; qs <- x::qs; y <@ RO.o(x); return y; }
+  proc hash = RO.o
 }.
 
 (* The initial scheme *)
 module S = Hashed_ElGamal(H).
 
+(*
 (* The reduction *)
-module SCDH_from_CPA(A:Adversary,O:Oracle): Top.SCDH.Adversary = {
+module SCDH_from_CPA(A:Adversary,O:Oracle): SCDHT.Adversary = {
   module BA = A(Bound(O))
 
   proc solve(gx:group, gy:group): group fset = {
@@ -102,16 +118,37 @@ module SCDH_from_CPA(A:Adversary,O:Oracle): Top.SCDH.Adversary = {
     return Log.qs;
   }
 }.
-
+*)
 (* We want to bound the probability of A winning CPA(Bounder(A,RO),S) in terms of
    the probability of B = CDH_from_CPA(SCDH_from_CPA(A,RO)) winning CDH(B) *)
+
+schema cost_eqnil ['a] `{P} {l:'a list} : cost [P: l = []] = cost [P:l] + 1.
+
+schema cost_empty ['a 'b] `{P} :
+  cost [P: empty<:'a, 'b>] = 1.
+
+(* FIXME *)
+schema cost_get ['a 'b] `{P} {m:('a, 'b) fmap, x:'a} :
+  cost [P: m.[x]] = cost[P:m] + cost[P:x] + 1.
+
+(* FIXME *)
+schema cost_set ['a 'b] `{P} {m:('a, 'b) fmap, x:'a, e:'b} :
+  cost [P: m.[x<-e]] = cost[P:m] + cost[P:x] + cost[P:e] + 1.
+
+(* FIXME *)
+schema cost_notin ['a 'b] `{P} {m:('a, 'b) fmap, x:'a} :
+  cost [P: x \notin m] = cost[P:m] + cost[P:x] + 1.
+
+schema cost_oget ['a] `{P} {o: 'a option} : 
+  cost [P : oget o] = cost [P:o] + 1.
+hint simplify cost_get, cost_set, cost_notin, cost_oget, cost_empty, cost_eqnil.
+
 section.
-  declare module A: Adversary {-RO, -Log, -OnBound.G1, -OnBound.G2}.
 
-  axiom choose_ll (O <: ARO {-A}): islossless O.o => islossless A(O).choose.
+  declare module A: Adversary [choose : `{cA.`cchoose, #O.o : cA.`ochoose},
+                               guess  : `{cA.`cguess,  #O.o : cA.`oguess}] {-H}.
+
   axiom guess_ll (O <: ARO {-A}) : islossless O.o => islossless A(O).guess.
-
-  local module BA = A(Bound(RO)).
 
   local module G0 = {
     var gxy:group
@@ -125,257 +162,111 @@ section.
       y       <$ dt;
       gx      <- g ^ x;
       gxy     <- gx ^ y;
-      (m0,m1) <@ BA.choose(gx);
-      b       <$ {0,1};
-      h       <@ H.hash(gxy);
-      c       <- (g ^ y, h +^ (b ? m1 : m0));
-      b'      <@ BA.guess(c);
-      return (b' = b);
-    }
-  }.
-
-  local equiv CPA_G0: CPA(S,BA).main ~ G0.main: ={glob A} ==> ={res}.
-  proof.
-    proc.
-    inline Hashed_ElGamal(H).kg Hashed_ElGamal(H).enc.
-    swap{1} 8 -5.
-    call (_: ={glob H, Log.qs}); first by sim.
-    wp; call (_: ={glob H}); first by sim.
-    wp; rnd.
-    call (_: ={glob H, Log.qs}); first by sim.
-    wp; do !rnd.
-    by call (_: true ==> ={glob H}); first by sim.
-  qed.
-
-  local lemma Pr_CPA_G0 &m:
-    Pr[CPA(S,BA).main() @ &m: res] = Pr[G0.main() @ &m: res]
-  by byequiv CPA_G0.
-
-  local module G1 = {
-    proc main() : bool = {
-      var m0, m1, c, b, b';
-      var x, y, h, gx, gxy;
-
-      H.init();
-      x       <$ dt;
-      y       <$ dt;
-      gx      <- g ^ x;
-      gxy     <- gx ^ y;
-      (m0,m1) <@ BA.choose(gx);
-      b       <$ {0,1};
-      h       <$ dbits;
-      c       <- (g ^ y, h +^ (b ? m1 : m0));
-      b'      <@ BA.guess(c);
-      return (b' = b);
-    }
-  }.
-
-  local module G2 = {
-    var gxy : group
-
-    proc main() : bool = {
-      var m0, m1, c, b, b';
-      var x, y, h, gx;
-
-      H.init();
-      x       <$ dt;
-      y       <$ dt;
-      gx      <- g ^ x;
-      gxy     <- gx ^ y;
-      (m0,m1) <@ BA.choose(gx);
-      b       <$ {0,1};
-      h       <$ dbits;
-      c       <- (g ^ y, h +^ (b ? m1 : m0));
-      b'      <@ BA.guess(c);
-      return G2.gxy \in Log.qs;
-    }
-  }.
-
-  local module (D : ROC.Dist) (H : ARO) = {
-    module A = A(H)
-
-    var y:t
-    var b:bool
-    var m0, m1:ptxt
-
-    proc a1(): group = {
-      var x, gxy, gx;
-
-      x       <$ dt;
-      y       <$ dt;
-      gx      <- g ^ x;
-      gxy     <- gx ^ y;
-      (m0,m1) <@ A.choose(gx);
-      b       <$ {0,1};
-      return gxy;
-    }
-
-    proc a2(x:bits): bool = {
-      var c, b';
-
-      c  <- (g ^ y, x +^ (b ? m1 : m0));
-      b' <@ A.guess(c);
-      return (b' = b);
-    }
-  }.
-
-  local lemma G0_D &m: Pr[G0.main() @ &m: res] = Pr[OnBound.G0(D,RO).main() @ &m: res].
-  proof.
-    byequiv (_: ={glob A} ==> ={res})=> //.
-    proc.
-    inline OnBound.G0(D,RO).D.a1 OnBound.G0(D,RO).D.a2; wp.
-    conseq (_: _ ==> ={b'} /\ b{1} = D.b{2})=> //.
-    by inline H.hash; sim.
-  qed.
-
-  local lemma G1_D &m: Pr[G1.main() @ &m: res] = Pr[OnBound.G1(D,RO).main() @ &m: res].
-  proof.
-    byequiv (_: ={glob A} ==> ={res})=> //.
-    proc.
-    inline OnBound.G1(D,RO).D.a1 OnBound.G1(D,RO).D.a2; wp.
-    conseq (_: _ ==> ={b'} /\ b{1} = D.b{2})=> //.
-    by inline H.hash; sim.
-  qed.
-
-  local lemma G2_D &m: Pr[G2.main() @ &m: res] = Pr[OnBound.G2(D,RO).main() @ &m: res].
-  proof.
-    byequiv (_: ={glob A} ==> ={res})=> //.
-    proc.
-    inline OnBound.G2(D,RO).D.a1 OnBound.G2(D,RO).D.a2; wp.
-    conseq (_: _ ==> ={glob Log, b'} /\ b{1} = D.b{2} /\ G2.gxy{1} = x{2})=> //.
-    by inline H.hash; sim.
-  qed.
-
-  local lemma G0_G1_G2 &m:
-    Pr[G0.main() @ &m: res] <= Pr[G1.main() @ &m: res] + Pr[G2.main() @ &m: res].
-  proof.
-    rewrite (G0_D &m) (G1_D &m) (G2_D &m).
-    apply (OnBound.ROM_BadCall D _ _ &m).
-    + move=> H0 H0_o_ll; proc; auto; call (choose_ll H0 _)=> //; auto=> />.
-      smt(dt_ll DBool.dbool_ll).
-    by progress; proc; call (guess_ll H _)=> //; auto.
-  qed.
-
-  local module G1' = {
-    proc main() : bool = {
-      var m0, m1, c, b, b';
-      var x, y, h, gx, gxy;
-
-      H.init();
-      x       <$ dt;
-      y       <$ dt;
-      gx      <- g ^ x;
-      gxy     <- gx ^ y;
-      (m0,m1) <@ BA.choose(gx);
-      b       <$ {0,1};
-      h       <$ dbits;
+      (m0,m1) <@ A(H).choose(gx);
+      h       <$ dbits; 
       c       <- (g ^ y, h);
-      b'      <@ BA.guess(c);
+      b'      <@ A(H).guess(c);
+      b       <$ {0,1};
       return (b' = b);
     }
   }.
 
-  local lemma G1_G1' &m: Pr[G1.main() @ &m: res] = Pr[G1'.main() @ &m: res].
+  local lemma Pr_CPA_G0 &m :
+    Pr[CPA(S,A(RO)).main() @ &m: res] <= 
+      Pr[G0.main() @ &m: res] + Pr[G0.main() @ &m: G0.gxy \in H.qs].
   proof.
-    byequiv (_: ={glob A} ==> ={res})=> //.
+    byequiv => //.
     proc.
-    call (_: ={glob RO, glob Log}); first by sim.
-    wp; rnd (fun h, h +^ if b then m1 else m0){1}; rnd.
-    call (_: ={glob RO, glob Log}); first by sim.
-    by inline H.init RO.init; auto=> /> *; split => *; algebra.
+    inline Hashed_ElGamal(H).kg Hashed_ElGamal(H).enc H.hash.
+    swap{1} 8 -5; swap{2} 10 -3.
+    call (_: G0.gxy \in H.qs, 
+            (forall x, x \in H.qs{2} = x \in RO.m{2}) /\
+            eq_except (pred1 G0.gxy{2}) RO.m{1} RO.m{2}).
+    + by apply guess_ll.
+    + proc; inline *; auto => /> &1 &2 hb; smt (eq_except_set_eq get_setE).
+    + by move=> *; islossless.
+    + by move=> /=; proc; call (_: true); 1: islossless; auto => />.
+    wp; rnd (fun y0 => y0 +^ m{1}) => /=.
+    wp; rnd; call (_: ={RO.m} /\ (forall x, x \in H.qs{2} = x \in RO.m{2})).
+    + by proc; inline *; auto => />; smt (get_setE).
+    inline *; auto => /> *; split; 1: by move=> *; rewrite mem_empty.
+    move=> _ ??? hdom ??; split; 1: by move=> *;ring.
+    smt(eq_except_setl get_setE).
   qed.
 
-  local lemma Pr_G1' &m: Pr[G1'.main() @ &m: res] = 1%r/2%r.
+  local lemma Pr_G0_res &m : 
+     Pr[G0.main() @ &m: res] <= 1%r/2%r.
   proof.
-    cut RO_o_ll:= RO_o_ll _; first by smt(dbits_ll).
-    byphoare (_: true ==> res)=> //.
-    proc.
-    swap 7 3.
-    rnd (pred1 b').
-    conseq (_: true) => />.
-    + by move=> b'; rewrite DBool.dbool1E /pred1 => />.
-    islossless.
-    + by apply (guess_ll (Bound(RO))); islossless.
-    by apply (choose_ll (Bound(RO))); islossless.
+    byphoare => //; proc.
+    rnd (pred1 b'); conseq (_:true) => //.
+    by move=> /> *; rewrite DBool.dbool1E.
   qed.
 
-  local module G2' = {
-    var gxy : group
-
-    proc main() : bool = {
-      var m0, m1, c, b, b';
-      var x, y, h, gx;
-
+  local module ALCDH = {
+    proc solve (gx:group, gy:group) : group list = {
+      var m0, m1, c, b';
+      var h;
       H.init();
-      x        <$ dt;
-      y        <$ dt;
-      gx       <- g ^ x;
-      gxy      <- gx ^ y;
-      (m0,m1)  <@ BA.choose(gx);
-      b        <$ {0,1};
-      h        <$ dbits;
-      c        <- (g ^ y, h);
-      b'       <@ BA.guess(c);
-      return gxy \in Log.qs;
+      (m0,m1) <@ A(H).choose(gx);
+      h       <$ dbits; 
+      c       <- (gy, h);
+      b'      <@ A(H).guess(c);
+      if (H.qs = []) H.qs <- [g];  
+      return H.qs;
     }
-  }.
+  }. 
 
-  local lemma G2_G2' &m: Pr[G2.main() @ &m: res] = Pr[G2'.main() @ &m: res].
+  local lemma cost_ALCDH : 
+     choare [ALCDH.solve : true ==> 0 < size res <= cA.`ochoose + cA.`oguess] 
+     time [6 + cunifin + (5 + cunifin) * (cA.`oguess + cA.`ochoose) + cA.`cguess + cA.`cchoose].
   proof.
-    byequiv (_: ={glob A} ==> ={res})=> //.
+    proc; wp.
+    call (_: true;
+           (H.o : size H.qs- cA.`ochoose)
+           time
+           [(H.o : [fun _ => 5 + cunifin])]).
+    + move=> zo hzo; proc; inline *.
+      by auto => &hr />; rewrite dbits_ll /=; smt().
+    auto; call (_: true;
+           (H.o : size H.qs)
+           time [(H.o : [fun _ => 5 + cunifin])]).
+    + move=> zo hzo; proc; inline *.
+      by auto => &hr />; rewrite dbits_ll /=; smt().
+    inline *; auto => />.
+    split => *.
+    + smt (dbits_ll size_ge0 size_eq0 cA_pos).
+    rewrite !bigi_constz /=; smt(cA_pos).
+  qed.
+
+  local lemma Pr_G0_LCDHPr_G0_res &m: 
+    Pr[G0.main() @ &m: G0.gxy \in H.qs] <= Pr[LCDH(ALCDH).main() @ &m : res].
+  proof.
+    byequiv => //.
     proc.
-    call (_: ={glob RO, glob Log}); first by sim.
-    wp; rnd (fun h, h +^ if b then m1 else m0){1}; rnd.
-    call (_: ={glob RO, glob Log}); first by sim.
-    by inline H.init RO.init; auto=> /> *; split => *; algebra.
+    conseq (_ : _ ==> G0.gxy{1} \in H.qs{1} => g ^ (x{2} * y{2}) \in s{2}) _ (_: true ==> size s <= qH) => //.
+    + by move=> />.
+    + call (_: true ==> 0 < size res <= qH); last by auto.
+      by conseq cost_ALCDH; smt (cA_pos).
+    inline *.
+    rnd{1}; auto; call (_: ={glob H}); 1: by sim.
+    auto; call (_: ={glob H}); 1: by sim.
+    by auto => /> *; rewrite -pow_pow.
   qed.
 
-  local equiv G2'_SCDH: G2'.main ~ SCDH(SCDH_from_CPA(A,RO)).main:
-    ={glob A} ==> res{1} = res{2} /\ card Log.qs{1} <= qH.
+  lemma ex_reduction &m : 
+    exists (B<:CDH.Adversary 
+      [solve : `{ C1.cduniform_n + 6 + cunifin + (5 + cunifin) * (cA.`oguess + cA.`ochoose) + cA.`cguess + cA.`cchoose}] {+A, +H}),
+    Pr[CPA(S,A(RO)).main() @ &m: res] - 1%r/2%r <= 
+    qH%r * Pr[CDH.CDH(B).main() @ &m: res].
   proof.
-    proc.
-    inline SCDH_from_CPA(A,RO).solve.
-    swap{2} 5 -4; swap{1} 7 3.
-    rnd{1}; wp.
-    seq  8  7: (={glob BA} /\
-                c{1} = (gy, h){2} /\
-                G2'.gxy{1} = g ^ (x * y){2} /\
-                card Log.qs{1} <= qH).
-      wp; rnd; call (_: ={glob H} /\ card Log.qs{1} <= qH).
-        proc; sp; if=> //; inline Bound(RO).LO.o RO.o; auto=> />.
-        by move=> &2 _ szqs_lt_qH _ _; rewrite fcardU fcard1; smt(fcard_ge0).
-      by inline H.init RO.init; auto=> />; rewrite fcards0; smt(gt0_qH pow_pow).
-    call (_: ={glob H} /\ card Log.qs{1} <= qH).
-      proc; sp; if=> //; inline Bound(RO).LO.o RO.o; auto=> /> &2 _ szqs_lt_qH _ _.
-      by rewrite fcardU fcard1; smt(fcard_ge0).
-    by auto => />.
+    have [B hB]:= C1.ex_reduction _ ALCDH &m cost_ALCDH.
+    exists B; split.
+    + proc true : time [] => // /#.
+    move: (Pr_CPA_G0 &m) (Pr_G0_res &m) (Pr_G0_LCDHPr_G0_res) => /#.
   qed.
 
-  local lemma Pr_G2'_SCDH &m :
-    Pr[G2'.main() @ &m: res]
-    = Pr[SCDH(SCDH_from_CPA(A,RO)).main() @ &m : res]
-  by byequiv G2'_SCDH.
-
-  local lemma Reduction &m :
-    Pr[CPA(S,BA).main() @ &m : res] <=
-    1%r / 2%r + Pr[SCDH(SCDH_from_CPA(A,RO)).main() @ &m : res].
-  proof.
-    rewrite (Pr_CPA_G0 &m).
-    rewrite -(Pr_G1' &m) -(G1_G1' &m).
-    rewrite -(Pr_G2'_SCDH &m) -(G2_G2' &m).
-    by apply (G0_G1_G2 &m).
-  qed.
-
-  (** Composing reduction from CPA to SCDH with reduction from SCDH to CDH *)
-  lemma Security &m:
-      Pr[CPA(S,A(Bound(RO))).main() @ &m: res] - 1%r / 2%r <=
-      qH%r * Pr[CDH.CDH(CDH_from_SCDH(SCDH_from_CPA(A,RO))).main() @ &m: res].
-  proof.
-    apply (ler_trans (Pr[SCDH(SCDH_from_CPA(A,RO)).main() @ &m: res])).
-    + smt(Reduction).
-    have:= Self.SCDH.Reduction (SCDH_from_CPA(A,RO)) &m gt0_qH.    
-    by rewrite -mulrA mul1r mulrC ler_pdivr_mulr 1:lt_fromint 1:gt0_qH mulrC.
-  qed.
 end section.
 
-print axiom Security.
+print ex_reduction.
+
+
